\documentclass{article}
\usepackage[utf8]{inputenc}
\usepackage{amsmath,amssymb,tikz-cd}

\usepackage[top=1cm, left=1 cm, right=1 cm,bottom=1.5 cm]{geometry}

\title{Thermodynamics fundamental relations}
\author{Keerthi vasan M}
\date{April 2022}

\begin{document}

\noindent \textbf{\Large DIFFERENTIAL FORM OF ENERGY PROPERTIES}\\[0.4cm]
Energy properties like $(U,H,G,\text{ and }A)$ are related to the reference properties $(P,T,V,\text{ and }S)$ as follows:\\[0.2 cm]
First law of thermodynamics: $dU = dQ + dW$ here $dW = -PdV$ and $dQ=TdS$. So,
\begin{equation} \label{U}
\begin{split}
    dU=TdS-PdV=U(S,V)
\end{split}
\end{equation}
 
\noindent Enthalpy $H$ is given by $H=U+PV$. Therefore,
\begin{equation} \label{H}
\begin{split}
    dH&=dU+d(PV) \\
    &=dU+PdV+VdP\\
    &=(TdS-PdV)+PdV+VdP \text{\ \ (Using equation (\ref{U}))}\\
    &=TdS+VdP\\
    \Rightarrow dH&=TdS+VdP=H(S,P)
\end{split}
\end{equation}
    
\noindent Gibb's free energy $G$ is given by $G=H-TS$. Therefore,  
\begin{equation} \label{G}
\begin{split}
    dG&=dH-d(TS) \\
    &=dH-TdS-SdT\\
    &=(TdS+VdP)-TdS-SdT \text{\ \ (Using equation (\ref{H}))}\\
    &=VdP-SdT\\
    \Rightarrow dG&=VdP-SdT=G(P,T)
\end{split}
\end{equation} 
    
\noindent Helmholtz free energy $A$ is given by $A=U-TS$. Therefore,  
\begin{equation} \label{A}
\begin{split}
    dA&=dU-d(TS) \\
    &=dU-TdS-SdT\\
    &=(TdS-PdV)-TdS-SdT \text{\ \ (Using equation (\ref{U}))}\\
    &=-PdV-SdT\\
    \Rightarrow dA&=-PdV-SdT=A(V,T)
\end{split}
\end{equation}
Now using the exact differential property of equation (\ref{U}) to (\ref{A}), we derive the well known Mazwell's equations as follows,
\begin{equation}
    \bigg(\frac{\partial T}{\partial V}\bigg)_S = -\bigg(\frac{\partial P}{\partial S}\bigg)_V,\ \  \bigg(\frac{\partial T}{\partial P}\bigg)_S = \bigg(\frac{\partial V}{\partial S}\bigg)_P ,\ \  \bigg(\frac{\partial V}{\partial T}\bigg)_P = -\bigg(\frac{\partial S}{\partial P}\bigg)_T,\ \  \bigg(\frac{\partial P}{\partial T}\bigg)_V = \bigg(\frac{\partial S}{\partial V}\bigg)_T
\end{equation}\\
\textbf{\Large MNEMONIC DIAGRAM}\\[0.4cm]

\begin{center}
\begin{tikzcd}
V \arrow[rr, "A", no head]                                        &  & T                                        \\
                                                                  &  &                                          \\
S \arrow[uu, "U", no head] \arrow[rr, "H"', no head] \arrow[rruu] &  & P \arrow[uu, "G"', no head] \arrow[lluu]
\end{tikzcd}    
\end{center}
\noindent
$V,T,P,S$ - ``\textbf{V}ijay's \textbf{T}uppakki is \textbf{P}akka \textbf{S}uperhit" and $A,G,H,U$ - Alphabetical order. Using the above diagram, derive the differential form of equation (\ref{U}) to (\ref{A}).

\end{document}
